src/Model.QUIC.fsti
@@ -253,7 +253,7 @@ val rframe_pnlog: #k:id{PNE.is_safe (snd k)} ->  #w:stream_writer k -> r:stream_
     M.loc_disjoint ri (rfootprint r))
   (ensures PNE.table (reader_pne_state r) h1 == l)
 
-val g_initial_packet_number: #k:id -> w: stream_writer k -> GTot pn
+val g_last_packet_number: #k:id -> #w: stream_writer k -> r:stream_reader w -> GTot (p:pn { p >= writer_offset w })
 
 val create: k:id -> u:info ->
   u1:AEAD.info (fst k) -> u2:PNE.info (snd k) -> init: pn ->
@@ -269,7 +269,6 @@ val create: k:id -> u:info ->
     writer_ae_info w == u1 /\
     writer_pne_info w == u2 /\
     writer_info w == u /\
-    g_initial_packet_number w == init /\
     (safe k ==>
       (AEAD.wlog (writer_aead_state w) h1 == Seq.empty /\
       PNE.table (writer_pne_state w) h1 == Seq.empty
@@ -292,7 +291,6 @@ val coerce: k:unsafe_id -> u:info ->
     writer_ae_info w == u1 /\
     writer_pne_info w == u2 /\
     writer_info w == u /\
-    g_initial_packet_number w == init /\
     writer_static_iv w ==
       Spec.derive_secret u1.AEAD.halg ts
         Spec.label_iv 12 /\
